Temporal_Planning_Base/Sequences.thy
@@ -1,0 +1,191 @@
+theory Sequences
+  imports Base
+begin
+definition "seq_apply fs x = map (\<lambda>i. (fold (id) (take i fs) x)) [1..<length fs + 1]"
+
+definition "ext_seq f xs \<equiv> xs @ f (last xs)"
+
+definition "ext_seq' fs xs = fold ext_seq fs xs"
+
+definition "seq_apply' fs x = tl (ext_seq' fs [x])"
+
+lemma length_seq_apply[simp]: 
+  "length (seq_apply fs s) = length fs"
+  unfolding seq_apply_def
+  apply (subst length_map)
+  apply (subst length_upt)
+  by simp
+
+lemma seq_apply_nth:
+  assumes "i < length fs"
+  shows "(seq_apply fs x) ! i = fold id (take (Suc i) fs) x"
+  unfolding seq_apply_def
+  apply (subst nth_map)
+  using assms apply simp
+  apply (subst nth_upt)
+  using assms apply simp
+  by auto
+
+lemma seq_apply_nth_Suc:
+  assumes "Suc i < length fs"
+  shows "(seq_apply fs s) ! (Suc i) = (fs ! (Suc i)) ((seq_apply fs s) ! i)"
+  apply (subst seq_apply_nth)
+  using assms apply simp
+  apply (subst seq_apply_nth)
+  using assms apply simp
+  apply (subst take_Suc_conv_app_nth)
+  using assms by auto
+
+lemma seq_apply_Cons_nth:
+  assumes "i \<le> length fs"
+  shows "(x#(seq_apply fs x)) ! i = fold id (take i fs) x"
+  apply (cases i)
+   apply simp
+  subgoal for i'
+    apply (simp)
+    apply (subst seq_apply_nth)
+    using assms by simp+
+  done   
+
+lemma seq_apply_Cons_nth_Suc:
+  assumes "i < length fs"
+  shows "(x#(seq_apply fs x)) ! (Suc i) = (fs ! i) ((x#(seq_apply fs x)) ! i)"
+  apply (subst nth_Cons_Suc)
+  apply (subst seq_apply_Cons_nth)
+  using assms apply simp
+  apply (subst seq_apply_nth)
+  using assms apply simp
+  apply (subst take_Suc_conv_app_nth[OF assms])
+  by simp
+
+lemma seq_apply_not_Nil:
+  assumes "fs \<noteq> []"
+  shows "seq_apply fs x \<noteq> []"
+  apply (subst length_greater_0_conv[symmetric])
+  using assms length_seq_apply 
+  by simp
+
+lemma seq_apply_Nil: "seq_apply [] x = []"
+  unfolding seq_apply_def by auto
+
+lemma last_seq_apply: 
+  assumes "fs \<noteq> []"
+  shows "last (seq_apply fs x) = fold id fs x"
+  apply (subst last_conv_nth)
+  using assms[THEN seq_apply_not_Nil] apply simp
+  apply (subst seq_apply_nth)
+  using assms apply simp
+  apply (subst take_all)
+  by simp+
+
+
+(* Precondition: the 0th state x must satisfy P *)
+(* The first state Q (fs ! 0) x must satisfy Q 0 *)
+(* Assuming the length of fs is 0, this is the final state *)
+(* Assuming the length of fs is greater than 0, this state satisfies P 1 *)
+(* the ith state (x#seq_apply fs x) ! i assuming i \<le> length fs*)
+(* Does the post-condition only have to hold when Suc i < length fs? Yes. We do not want 
+a vacuous post-condition to hold *)
+(* The pre to post condition. The final state is (fs ! (length fs - 1)) s 
+  For this, we want *)
+context
+  fixes fs::"('a \<Rightarrow> 'a) list"
+    and P Q::"nat \<Rightarrow>'a \<Rightarrow> bool"
+    and R::"'a \<Rightarrow> bool"
+    and S::"'a \<Rightarrow> bool"
+  assumes PQ: "\<And>i s. i < length fs \<Longrightarrow> P i s \<Longrightarrow> (Q i ((fs ! i) s))"
+      and QP: "\<And>i s. Suc i < length fs \<Longrightarrow> Q i s \<Longrightarrow> P (Suc i) s"
+begin
+
+(* The implications only hold when there are actual functions.
+  Therefore, we need to first consider cases in which there are some functions *)
+lemma seq_apply_pre_post_induct_steps_pre:
+  assumes i: "i < length fs"
+      and Px0: "P 0 x"
+    shows "P i ((x#seq_apply fs x) ! i)"
+  using i
+proof (induction i)
+  case 0
+  then show ?case using Px0 by simp
+next
+  case (Suc i)
+  hence i: "i < length fs" by simp
+  show ?case 
+    apply (rule QP[OF Suc(2)])
+    apply (subst seq_apply_Cons_nth_Suc[OF i])
+    apply (rule PQ[OF i])
+    using Suc by simp
+qed
+
+lemma seq_apply_pre_post_induct_steps_post:
+  assumes i: "i < length fs"
+      and Px0: "P 0 x"
+    shows "Q i ((x#seq_apply fs x) ! (Suc i))"
+  apply (subst seq_apply_Cons_nth_Suc[OF i])
+  apply (rule PQ[OF i])
+  by (rule seq_apply_pre_post_induct_steps_pre[OF assms])
+
+
+lemma seq_apply_pre_post_induct_length_post:
+  assumes l: "0 < length fs"
+      and Px0: "P 0 x"
+    shows "Q (length fs - 1) (last (x#seq_apply fs x))"
+proof - 
+  have "Q (length fs - 1) ((x # seq_apply fs x) ! Suc (length fs - 1))" 
+    using seq_apply_pre_post_induct_steps_post[of "length fs - 1", OF _ Px0] l by simp
+  thus ?thesis
+    apply (subst (asm) seq_apply_Cons_nth)
+    using assms apply simp
+    apply (subst last_conv_nth)
+     apply simp
+    apply (subst seq_apply_Cons_nth)
+    using assms apply simp
+    apply (subst take_all)
+     apply simp
+    apply (subst (asm) take_all)
+    by simp+
+qed
+ 
+lemma seq_apply_pre_post_induct_weaken_pre_strengthen_post:
+  assumes i: "i \<le> length fs"
+      and Rx0: "R x"
+      and RP0: "\<And>x. 0 < length fs \<Longrightarrow> R x \<Longrightarrow> P 0 x"
+      and QSl: "\<And>x. Q (length fs - 1) x \<Longrightarrow> S x"
+      and RS0: "\<And>x. 0 = length fs \<Longrightarrow> R x \<Longrightarrow> S x"
+    shows "S (last (x#seq_apply fs x))"
+  apply (cases fs)
+  subgoal 
+    apply (rule ssubst[of fs], assumption)
+    apply (subst seq_apply_Nil)
+    using RS0 Rx0 by simp
+  subgoal for f fs'
+    apply (rule QSl)
+    apply (rule seq_apply_pre_post_induct_length_post)
+     apply simp
+    apply (rule RP0)
+     apply simp
+    by (rule Rx0)
+  done
+
+end
+
+context
+  fixes fs::"('a \<Rightarrow> 'a list) list"
+  assumes f_wf: "\<And>f x. f \<in> set fs \<Longrightarrow> f x \<noteq> []"
+begin
+thm ext_seq'_def
+
+end
+
+context 
+  fixes fs::"('a \<Rightarrow> 'a list) list"
+      and P Q::"nat \<Rightarrow>'a \<Rightarrow> bool"
+      and R::"'a \<Rightarrow> bool"
+      and S::"'a \<Rightarrow> bool"
+  assumes f_wf: "\<forall>f \<in> set fs. \<forall>x. f x \<noteq> []"
+      and PQ: "\<forall>i < length fs. \<forall>s. P i s \<longrightarrow> (Q i (last ((fs ! i) s)))"
+      and QP: "\<forall>i < length fs - 1. \<forall>s. Q i s\<longrightarrow> P (Suc i) s"
+begin
+
+end
+end
